src/3d/Main.fst
@@ -213,40 +213,18 @@ let emit_fstar_code_for_interpreter (en:env)
       let external_api_fsti_file =
         open_write_file
           (Printf.sprintf "%s/%s.ExternalAPI.fsti" (Options.get_output_dir ()) modul) in
-      FStar.IO.write_string external_api_fsti_file (Target.print_external_api_fstar modul tds);
+      FStar.IO.write_string external_api_fsti_file (Target.print_external_api_fstar_interpreter modul tds);
       FStar.IO.close_write_file external_api_fsti_file
     end;
-
-    let fsti_file =
-      open_write_file
-        (Printf.sprintf "%s/%s.fsti"
-          (Options.get_output_dir())
-          modul) in
-    FStar.IO.write_string fsti_file
-      (FStar.Printf.sprintf "module %s\n\
-                             open EverParse3d.Prelude\n\
-                             open EverParse3d.Actions.All\n\
-                             open EverParse3d.Interpreter\n\
-                             module T = FStar.Tactics\n\
-                             module A = EverParse3d.Actions.All\n\
-                             module P = EverParse3d.Prelude\n"
-                             modul);
-    FStar.IO.write_string fsti_file iface;
-    FStar.IO.close_write_file fsti_file;
-
-
-    let fst_file =
-      open_write_file
-        (Printf.sprintf "%s/%s.fst"
-          (Options.get_output_dir())
-          modul) in
+ 
     let maybe_open_external_api =
       if has_external_api
       then Printf.sprintf "open %s.ExternalAPI" modul
       else ""
     in
-    FStar.IO.write_string fst_file 
-      (FStar.Printf.sprintf "module %s\n\
+ 
+    let module_prefix = 
+       FStar.Printf.sprintf "module %s\n\
                              open EverParse3d.Prelude\n\
                              open EverParse3d.Actions.All\n\
                              open EverParse3d.Interpreter\n\
@@ -258,7 +236,25 @@ let emit_fstar_code_for_interpreter (en:env)
                              #push-options \"--using_facts_from 'Prims FStar.UInt FStar.UInt8 \
                                                                  FStar.UInt16 FStar.UInt32 FStar.UInt64 \
                                                                  EverParse3d FStar.Int.Cast %s'\"\n"
-                             modul maybe_open_external_api (all_modules |> String.concat " "));
+                             modul maybe_open_external_api (all_modules |> String.concat " ")
+    in
+                             
+    let fsti_file =
+      open_write_file
+        (Printf.sprintf "%s/%s.fsti"
+          (Options.get_output_dir())
+          modul) in
+    FStar.IO.write_string fsti_file module_prefix;
+    FStar.IO.write_string fsti_file iface;
+    FStar.IO.close_write_file fsti_file;
+
+
+    let fst_file =
+      open_write_file
+        (Printf.sprintf "%s/%s.fst"
+          (Options.get_output_dir())
+          modul) in
+    FStar.IO.write_string fst_file module_prefix;
     FStar.IO.write_string fst_file impl;    
     FStar.IO.close_write_file fst_file
 
